WIP in inline proof

theories/L6_PCPS/inline_correct.v
@@ -554,28 +554,58 @@ Section Inline_correct.
       inv H0. eapply H1 in H. inv H. contradiction. inv H0; eauto.
     - right. rewrite add_fundefs_not_in in H. do 4 eexists; split; eauto.
       eassumption.
-  Qed. 
+  Qed.
 
+  Lemma funname_in_exp_subset_mut :
+    (forall e, funname_in_exp e \subset bound_var e) /\
+    (forall B, funname_in_fundefs B \subset bound_var_fundefs B).
+  Proof.
+    exp_defs_induction IHe IHl IHB; intros; normalize_bound_var; simpl; sets.
+
+    eapply Union_Included. eapply Union_Included. now sets.
+    eapply Included_trans. eapply name_in_fundefs_bound_var_fundefs. sets.
+    sets.
+  Qed.
+
+  Lemma funname_in_exp_subset :
+    forall e, funname_in_exp e \subset bound_var e.
+  Proof. eapply funname_in_exp_subset_mut. Qed.
+
+  Lemma funname_in_fundefs_subset :
+    forall e, funname_in_fundefs e \subset bound_var_fundefs e.
+  Proof. eapply funname_in_exp_subset_mut. Qed.
+
+
+  Lemma fun_in_fundefs_bound_var_Setminus' e f ft xs B :
+    fun_in_fundefs B (f, ft, xs, e) ->
+    unique_bindings_fundefs B ->
+    bound_var e \\ funname_in_exp e \subset bound_var_fundefs B \\ funname_in_fundefs B \\ name_in_fundefs B.
+  Proof.
+    intros Hin Hun. induction B; [| now inv Hin ].
+    inv Hun. simpl in Hin. inv Hin.
+    - inv H. simpl. normalize_bound_var. rewrite !Setminus_Union_distr. do 2 eapply Included_Union_preserv_r.
+      eapply Included_Union_preserv_l. eapply Included_Setminus.
+      + eapply Union_Disjoint_r. eapply Disjoint_Singleton_r. now intros Hc; inv Hc; eauto.
+        eapply Disjoint_Included_r. eapply name_in_fundefs_bound_var_fundefs. sets.
+      + rewrite <- Setminus_Union. eapply Included_Setminus; [| now sets ].
+        eapply Disjoint_Included_r. eapply funname_in_fundefs_subset. sets.
+    - eapply Included_trans. eapply IHB; eauto.
+      simpl. normalize_bound_var. rewrite !Setminus_Union_distr. do 3 eapply Included_Union_preserv_r.
+      rewrite !Setminus_Union. rewrite <- !Union_assoc. rewrite (Union_commut (funname_in_exp _)). rewrite (Union_commut [set v]).
+      rewrite <- !Union_assoc. rewrite Union_assoc. do 2 rewrite <- Setminus_Union. 
+      eapply Included_Setminus; [| now sets ]. eapply Union_Disjoint_r.
+      eapply Disjoint_Singleton_r. now intros Hc; inv Hc; inv H0; eauto.
+      eapply Disjoint_Included_r. eapply funname_in_exp_subset. sets.
+  Qed.
 
   Lemma fun_in_fundefs_bound_var_Setminus e f ft xs B :
     fun_in_fundefs B (f, ft, xs, e) ->
     unique_bindings_fundefs B ->
     bound_var e \\ funname_in_exp e \subset bound_var_fundefs B \\ funname_in_fundefs B.
   Proof.
-    intros Hin Hun. induction B; [| now inv Hin ].
-    inv Hun. simpl in Hin. inv Hin.
-    - inv H. simpl. normalize_bound_var.
-  Admitted.
-
-  Lemma fun_in_fundefs_bound_var_Setminus' e f ft xs B :
-    fun_in_fundefs B (f, ft, xs, e) ->
-    unique_bindings_fundefs B ->
-    bound_var e \\ funname_in_exp e \\ name_in_fundefs B \subset bound_var_fundefs B \\ funname_in_fundefs B.
-  Proof.
-    intros Hin Hun. induction B; [| now inv Hin ].
-    inv Hun. simpl in Hin. inv Hin.
-    - inv H. simpl. normalize_bound_var.
-  Admitted.
+    intros Hin Hun. eapply Included_trans. eapply fun_in_fundefs_bound_var_Setminus'. eassumption.
+    eassumption. sets.
+  Qed.
 
 
   Lemma fun_in_fundefs_FromList_subset e f ft xs B :
@@ -583,9 +613,22 @@ Section Inline_correct.
     unique_bindings_fundefs B ->
     FromList xs \subset bound_var_fundefs B \\ funname_in_fundefs B \\ name_in_fundefs B.
   Proof.
-    intros Hin Hun. induction B; [| now inv Hin ]. inv Hin.
-    - inv H. normalize_bound_var. simpl.
-  Admitted.    
+    intros Hin Hun. induction B; [| now inv Hin ]. inv Hun. inv Hin.
+    - inv H. simpl. normalize_bound_var. rewrite !Setminus_Union_distr. eapply Included_Union_preserv_r.
+      eapply Included_Union_preserv_l. rewrite !Setminus_Union. eapply Included_Setminus; [| now sets ].
+      eapply Union_Disjoint_r; eapply Union_Disjoint_r.
+      + eapply Disjoint_Included_r. eapply funname_in_exp_subset. sets.
+      + eapply Disjoint_Included_r. eapply funname_in_fundefs_subset. sets.
+      + sets.
+      + eapply Disjoint_Included_r. eapply name_in_fundefs_bound_var_fundefs. sets.
+    - eapply Included_trans. eapply IHB; eauto.
+      simpl. normalize_bound_var. rewrite !Setminus_Union_distr. do 3 eapply Included_Union_preserv_r.
+      rewrite !Setminus_Union. rewrite <- !Union_assoc. rewrite (Union_commut (funname_in_exp _)). rewrite (Union_commut [set v]).
+      rewrite <- !Union_assoc. rewrite Union_assoc. do 2 rewrite <- Setminus_Union. 
+      eapply Included_Setminus; [| now sets ]. eapply Union_Disjoint_r.
+      eapply Disjoint_Singleton_r. now intros Hc; inv Hc; inv H0; eauto.
+      eapply Disjoint_Included_r. eapply funname_in_exp_subset. sets.
+  Qed.
 
   Lemma bound_var_fun_map_get f ft xs e (fm : fun_map) :
     M.get f fm = Some (ft, xs, e) ->
@@ -623,48 +666,97 @@ Section Inline_correct.
   (*     eassumption. *)
   (* Qed.  *)
 
+  (* TODO move *)
+  Lemma preord_env_P_inj_set_extend_not_In_P_r_alt S k f rho1 rho2 x y v :
+    preord_env_P_inj cenv PG S k f rho1 rho2 ->
+    ~ x \in Dom_map rho1 ->
+    ~ y \in (image f (Dom_map rho1)) ->
+    preord_env_P_inj cenv PG S k (f {x ~> y}) rho1 (M.set y v rho2).
+  Proof.
+    intros Henv Hnin Hnin' z Hy v' Hget.
+    edestruct Henv as [v'' [Hget' Hv]]; eauto.
+    eexists; split; eauto.
+    rewrite extend_gso, M.gso. eassumption.
+    intros Hc; subst. eapply Hnin'. eexists; eauto. split. eexists; eauto. reflexivity.
+    intros Hc. subst. eapply Hnin. eexists. eassumption.
+  Qed.  
+
+  Lemma Dom_map_add_fundefs fm B :
+    Dom_map (add_fundefs B fm) <--> name_in_fundefs B :|: Dom_map fm.
+  Proof.
+    induction B; simpl; [| now sets ].
+    rewrite Dom_map_set. rewrite IHB. sets.
+  Qed.
+
+  
+  Lemma sub_map_def_funs rho B :
+    Disjoint _ (name_in_fundefs B) (Dom_map rho) ->            
+    sub_map rho (def_funs B B rho rho).
+  Proof.
+    intros Hdis x v Hget.
+    rewrite def_funs_neq; eauto.
+    intros Hc. eapply Hdis. constructor. eassumption. eexists. eassumption.
+  Qed.
+
+  Lemma Dom_map_def_funs B rho B' rho' :
+    Dom_map (def_funs B' B rho' rho) <--> name_in_fundefs B :|: Dom_map rho. 
+  Proof.
+    induction B; simpl; sets.
+    rewrite Dom_map_set. rewrite IHB. sets.
+  Qed.
+
+  Lemma Dom_map_sub_map {A : Type} (rho1 rho2 : M.t A) :
+    sub_map rho1 rho2 ->
+    Dom_map rho1 \subset Dom_map rho2.
+  Proof.
+    intros H1 x [y Hin]. eapply H1 in Hin.
+    eexists; eauto.
+  Qed.
+
 
   Lemma fun_map_inv_set_not_In_r k S fm rho1 rho2 i sig x x' v' : 
     fun_map_inv k S fm rho1 rho2 i sig ->
-    ~ x \in occurs_free_fun_map fm ->
-    ~ x' \in image (apply_r sig) (occurs_free_fun_map fm) ->
+    ~ x \in (Dom_map rho1) ->
+    ~ x' \in image (apply_r sig) (Dom_map rho1) ->
     fun_map_inv k S fm rho1 (M.set x' v' rho2) i (M.set x x' sig).
   Proof.
     revert S fm rho1 rho2 i sig x x' v'. induction k using lt_wf_rec1; intros. intro; intros.
-    edestruct H0; eauto.
+    edestruct H0; eauto. 
     destructAll. split; [| split; [| split; [| split; [| split; [| split ]]]]]; eauto.
-    - rewrite apply_r_set_f_eq. eapply preord_env_P_inj_set_extend_not_In_P_r. eassumption.
-      + intros Hc. eapply H1. eapply occurs_free_fun_map_get; eassumption.
-      + intros Hc. eapply H2. eapply image_monotonic; [| eassumption ]. 
-        eapply occurs_free_fun_map_get; eauto.
+    - rewrite apply_r_set_f_eq. eapply preord_env_P_inj_set_extend_not_In_P_r_alt. eassumption.
+      + intros Hc. eapply H1. eapply Dom_map_sub_map. eassumption. eassumption.
+      + intros Hc. eapply H2. eapply image_monotonic; [| eassumption ].
+        eapply Dom_map_sub_map; eassumption.
     - destruct k; eauto. rewrite <- fun_map_inv_eq in *.
-      eapply H. omega. eassumption. eassumption. eassumption.
+      eapply H. omega. eassumption.
+      intros hc. eapply H1. eapply Dom_map_sub_map. eassumption. eassumption.
+      intros hc. eapply H2. eapply image_monotonic; [| eassumption ]. eapply Dom_map_sub_map. eassumption.
   Qed.
   
   Lemma fun_map_inv_set k S fm rho1 rho2 i sig x v x' v' :
     fun_map_inv k S fm rho1 rho2 i sig ->
-    ~ x \in Dom_map rho1 :|: Dom_map fm :|: occurs_free_fun_map fm ->
-    ~ x' \in image (apply_r sig) (occurs_free_fun_map fm) ->
+    ~ x \in Dom_map rho1 :|: Dom_map fm ->
+    ~ x' \in image (apply_r sig) (Dom_map rho1) ->
     fun_map_inv k (x |: S) fm (M.set x v rho1) (M.set x' v' rho2) i (M.set x x' sig).
   Proof.
     intros Hinv Hnin Hnin'. intro; intros.
     rewrite M.gso in *. 
-    2:{ intros Heq; subst. eapply Hnin. left. right. eexists; eauto. }
+    2:{ intros Heq; subst. eapply Hnin. right. eexists; eauto. }
     inv H.
-    - inv H2. exfalso. eapply Hnin. left. left. eexists; eauto.
+    - inv H2. exfalso. eapply Hnin. left. eexists; eauto.
     - edestruct Hinv; eauto.
       destructAll. split; [| split; [| split; [| split; [| split; [| split ]]]]]; eauto.
-      + rewrite apply_r_set_f_eq. eapply preord_env_P_inj_set_extend_not_In_P_r. eassumption.
-        intros Hc. eapply Hnin. right. eapply occurs_free_fun_map_get; eassumption. simpl.
-        intros Hc. eapply Hnin'. eapply image_monotonic; [| eassumption ].
-        eapply occurs_free_fun_map_get; eassumption.
+      + rewrite apply_r_set_f_eq. eapply preord_env_P_inj_set_extend_not_In_P_r_alt. eassumption.
+        intros Hc. eapply Hnin. left. eapply Dom_map_sub_map. eassumption. eassumption.
+        intros Hc. eapply Hnin'. eapply image_monotonic; [| eassumption ]. eapply Dom_map_sub_map. eassumption.
       + eapply sub_map_trans. eassumption. eapply sub_map_set.
-        intros Hc. eapply Hnin. left. left. eassumption.
+        intros Hc. eapply Hnin. left. eassumption.
       + destruct k; eauto. rewrite <- fun_map_inv_eq in *.
         eapply fun_map_inv_set_not_In_r. eapply fun_map_inv_antimon. eassumption.
         * reflexivity.
-        * intros Hc. eapply Hnin. right. eassumption.
-        * intros Hc. eapply Hnin'. eapply image_monotonic; [| eassumption ]. sets.
+        * intros Hc. eapply Hnin. left. eapply Dom_map_sub_map. eassumption. eassumption.
+        * intros Hc. eapply Hnin'. eapply image_monotonic; [| eassumption ].
+          eapply Dom_map_sub_map. eassumption.
   Qed.
   
 (* 
@@ -723,11 +815,36 @@ Section Inline_correct.
     eapply apply_r_set_f_eq. eapply f_eq_extend. eauto.
   Qed.
 
+  Lemma preord_env_P_inj_extend_not_In_P_r_alt k S σ rho1 rho2 x y :
+    preord_env_P_inj cenv PG S k σ rho1 rho2 -> 
+    ~ x \in Dom_map rho1 ->
+    preord_env_P_inj cenv PG S k (σ {x ~> y}) rho1 rho2.
+  Proof.
+    intros Hpre Hnin z Hp v1 Hget.
+    edestruct Hpre as [v2 [Hget2 Hpre2]]; eauto.
+    repeat eexists; eauto. rewrite extend_gso; eauto.
+    intros Hc. subst. apply Hnin. eexists; eauto.
+  Qed.
+
+
+  Lemma preord_env_P_inj_extend_lst_not_In_P_r_alt k S σ rho1 rho2 xs ys:
+    preord_env_P_inj cenv PG S k σ rho1 rho2 -> 
+    Disjoint _ (FromList xs) (Dom_map rho1) ->
+    preord_env_P_inj cenv PG S k (σ <{xs ~> ys}>) rho1 rho2.
+  Proof.
+    revert k S σ rho1 rho2 ys. induction xs; intros.
+    - simpl. eassumption.
+    - destruct ys. eassumption.
+      repeat normalize_sets. simpl. eapply preord_env_P_inj_extend_not_In_P_r_alt.
+      eapply IHxs. eassumption. now sets.
+      intros Hc. eapply H0. constructor; eauto.
+  Qed.
+
 
   Lemma fun_map_inv_sig_extend_Disjoint k S fm rho1 rho2 i sig xs xs' :
     fun_map_inv k S fm rho1 rho2 i sig ->
 
-    Disjoint _ (FromList xs) (occurs_free_fun_map fm) ->    
+    Disjoint _ (FromList xs) (Dom_map rho1) ->    
     
     fun_map_inv k S fm rho1 rho2 i (set_list (combine xs xs') sig).
   Proof.
@@ -736,14 +853,16 @@ Section Inline_correct.
     intro; intros. edestruct Hfm; eauto. destructAll.
     split; eauto. split; eauto. split; [| split; [| split; [| split ]]].
     - rewrite apply_r_set_list_f_eq. 
-      eapply preord_env_P_inj_extend_lst_not_In_P_r. eassumption.
-      eapply Disjoint_Included_r; [| eapply Hdis1 ].
-      eapply occurs_free_fun_map_get; eauto.
+      eapply preord_env_P_inj_extend_lst_not_In_P_r_alt. eassumption.
+      eapply Disjoint_Included_r; [| eapply Hdis1 ]. 
+      eapply Dom_map_sub_map. eassumption.
     - eassumption.
     - eassumption.
     - eassumption.
     - destruct k; eauto. rewrite <- fun_map_inv_eq in *. eapply H. omega.
-      eassumption. sets.
+      eassumption.
+      eapply Disjoint_Included_r; [| eapply Hdis1 ]. 
+      eapply Dom_map_sub_map. eassumption.
   Qed.
 
   Lemma fun_map_inv_set_lists k S fm rho1 rho1' rho2 i sig xs vs :
@@ -776,19 +895,19 @@ Section Inline_correct.
   Lemma preord_env_P_inj_set_lists_not_In_P_r S k f rho1 rho2 rho2' xs vs :
     preord_env_P_inj cenv PG S k f rho1 rho2 ->
     set_lists xs vs rho2 = Some rho2' ->
-    Disjoint _(FromList xs) (image f S) ->
+    Disjoint _(FromList xs) (image f (Dom_map rho1)) ->
     preord_env_P_inj cenv PG S k f rho1 rho2'.
   Proof.
     intros Henv Hnin Hnin' z Hy v' Hget.
     edestruct Henv as [v'' [Hget' Hv]]; eauto.
     eexists; split; eauto. erewrite <- set_lists_not_In. eassumption.
     eassumption. intros Hc. eapply Hnin'. constructor. eassumption.
-    eapply In_image. eassumption.
+    eapply In_image. eexists; eauto.
   Qed.
 
   Lemma fun_map_inv_set_lists_r k S fm rho1 rho2' rho2 i sig xs vs :
     fun_map_inv k S fm rho1 rho2 i sig ->
-    Disjoint _ (FromList xs) (image (apply_r sig) (occurs_free_fun_map fm)) ->    
+    Disjoint _ (FromList xs) (image (apply_r sig) (Dom_map rho1)) ->    
 
     set_lists xs vs rho2 = Some rho2' ->
     
@@ -800,48 +919,31 @@ Section Inline_correct.
     intro f; intros.
     edestruct Hfm; eauto. destructAll. split; eauto. split; eauto. split; [| split; [| split; [| split ]]]; try eassumption.
     + eapply preord_env_P_inj_set_lists_not_In_P_r. eassumption. eassumption.
-      eapply Disjoint_Included_r; [| eassumption ]. eapply image_monotonic. eapply occurs_free_fun_map_get. eassumption.
+      eapply Disjoint_Included_r; [| eassumption ]. eapply image_monotonic. eapply Dom_map_sub_map. eassumption.
     + destruct k; eauto. rewrite <- fun_map_inv_eq in *.
-      eapply H. omega. eassumption. eassumption. eassumption.
+      eapply H. omega. eassumption.
+      eapply Disjoint_Included_r; [| eapply Hdis1 ]. eapply image_monotonic. eapply Dom_map_sub_map. eassumption.
+      eassumption.
   Qed.
-
-  Lemma Dom_map_add_fundefs fm B :
-    Dom_map (add_fundefs B fm) <--> name_in_fundefs B :|: Dom_map fm.
-  Proof.
-    induction B; simpl; [| now sets ].
-    rewrite Dom_map_set. rewrite IHB. sets.
-  Qed.
-
   
-  Lemma sub_map_def_funs rho B :
-    Disjoint _ (name_in_fundefs B) (Dom_map rho) ->            
-    sub_map rho (def_funs B B rho rho).
-  Proof.
-    intros Hdis x v Hget.
-    rewrite def_funs_neq; eauto.
-    intros Hc. eapply Hdis. constructor. eassumption. eexists. eassumption.
-  Qed.
-
-  Lemma Dom_map_def_funs B rho B' rho' :
-    Dom_map (def_funs B' B rho' rho) <--> name_in_fundefs B :|: Dom_map rho. 
-  Proof.
-    induction B; simpl; sets.
-    rewrite Dom_map_set. rewrite IHB. sets.
-  Qed.
-
-  Lemma Dom_map_sub_map {A : Type} (rho1 rho2 : M.t A) :
-    sub_map rho1 rho2 ->
-    Dom_map rho1 \subset Dom_map rho2.
-  Proof.
-    intros H1 x [y Hin]. eapply H1 in Hin.
+  Lemma preord_env_P_inj_def_funs_neq_r_alt S k σ rho1 rho2 B0 B :
+    preord_env_P_inj cenv PG S k σ rho1 rho2->
+    Disjoint _ (image σ (Dom_map rho1)) (name_in_fundefs B) ->
+    preord_env_P_inj cenv PG S k σ rho1 (def_funs B0 B rho2 rho2).
+  Proof. 
+    intros Henv Hd x Hin v Hget.
+    rewrite def_funs_neq. now eapply Henv.
+    intros Hc. eapply Hd. constructor; eauto. eapply In_image.
     eexists; eauto.
   Qed.
+
+
 
   Lemma fun_map_inv_add_fundefs_Disjoint k S fm rho1 rho2 i sig B1 B2 :
     fun_map_inv k S fm rho1 rho2 i sig ->
     
-    Disjoint _ (name_in_fundefs B1) (S :|: Dom_map rho1 :|: occurs_free_fun_map fm) ->
-    Disjoint _ (name_in_fundefs B2) (image (apply_r sig) (occurs_free_fun_map fm)) ->
+    Disjoint _ (name_in_fundefs B1) (Dom_map rho1) ->
+    Disjoint _ (name_in_fundefs B2) (image (apply_r sig) (Dom_map rho1)) ->
 
     fun_map_inv k S (add_fundefs B1 fm) rho1 (def_funs B2 B2 rho2 rho2) i
                 (set_list (combine (all_fun_name B1) (all_fun_name B2)) sig).
@@ -850,50 +952,28 @@ Section Inline_correct.
     intro; intros. rewrite add_fundefs_not_in in H4.
     edestruct H0; eauto. destructAll.
     repeat (split; [ now eauto |]). split; [| split; [| split; [| split ]]].
-    - eapply preord_env_P_inj_def_funs_neq_r.
-      rewrite apply_r_set_list_f_eq. eapply preord_env_P_inj_extend_lst_not_In_P_r.
+    - eapply preord_env_P_inj_def_funs_neq_r_alt.
+      rewrite apply_r_set_list_f_eq. eapply preord_env_P_inj_extend_lst_not_In_P_r_alt.
       eassumption. rewrite <- Same_set_all_fun_name.
-      eapply Disjoint_Included_r. eapply occurs_free_fun_map_get. eassumption. sets.
+      eapply Disjoint_Included_r. eapply Dom_map_sub_map. eassumption. now sets. 
       rewrite apply_r_set_list_f_eq. eapply Disjoint_Included_l.
       intros x Hc. destruct Hc. destructAll.
       rewrite extend_lst_gso. eapply In_image. eassumption.
       rewrite <- Same_set_all_fun_name. intros Hc. eapply H1. constructor. eassumption.
-      right. eapply occurs_free_fun_map_get. eassumption. eassumption.
+      eapply Dom_map_sub_map; eassumption.
       eapply Disjoint_sym. eapply Disjoint_Included_r; [| eassumption ]. eapply image_monotonic.
-      eapply occurs_free_fun_map_get. eassumption. 
+      eapply Dom_map_sub_map. eassumption.
     - eassumption.
     - eassumption.
     - sets.
     - destruct k; eauto. rewrite <- fun_map_inv_eq in *. eapply H. 
       + omega.
       + eassumption.
-      + eapply Disjoint_Included_r; [| eassumption ]. eapply Union_Included. eapply Union_Included.
-        * eapply Included_trans. eapply occurs_free_fun_map_get. eassumption. sets.
-        * eapply Included_trans. eapply Dom_map_sub_map. eassumption. sets.
-        * sets.
-      + sets.
-    - intros Hc. eapply H1. constructor. eassumption. do 2 left. eassumption.
+      + eapply Disjoint_Included_r; [| eassumption ]. eapply Dom_map_sub_map. eassumption.
+      + eapply Disjoint_Included_r; [| eassumption ]. eapply image_monotonic.
+        eapply Dom_map_sub_map. eassumption.
+    - intros Hc. eapply H1. constructor. eassumption. eexists; eauto.  
   Qed.
-
-
-  Lemma funname_in_exp_subset_mut :
-    (forall e, funname_in_exp e \subset bound_var e) /\
-    (forall B, funname_in_fundefs B \subset bound_var_fundefs B).
-  Proof.
-    exp_defs_induction IHe IHl IHB; intros; normalize_bound_var; simpl; sets.
-
-    eapply Union_Included. eapply Union_Included. now sets.
-    eapply Included_trans. eapply name_in_fundefs_bound_var_fundefs. sets.
-    sets.
-  Qed.
-
-  Lemma funname_in_exp_subset :
-    forall e, funname_in_exp e \subset bound_var e.
-  Proof. eapply funname_in_exp_subset_mut. Qed.
-
-  Lemma funname_in_fundefs_subset :
-    forall e, funname_in_fundefs e \subset bound_var_fundefs e.
-  Proof. eapply funname_in_exp_subset_mut. Qed.
 
   Lemma name_in_fundefs_funname_in_fundefs_Disjoint B1 : 
     unique_bindings_fundefs B1 ->
@@ -920,15 +1000,16 @@ Section Inline_correct.
     occurs_free_fundefs B1 \subset S ->
     
     Disjoint _ (bound_var_fundefs B1) (Dom_map rho1) ->
-    Disjoint _ (bound_var_fundefs B1 \\ funname_in_fundefs B1) (occurs_free_fun_map fm) ->
+    Disjoint _ (name_in_fundefs B2) (image (apply_r sig) (Dom_map rho1)) ->
+        
+    (* Disjoint _ (bound_var_fundefs B1 \\ funname_in_fundefs B1) (occurs_free_fun_map fm) -> *)
 
-    Disjoint _ (name_in_fundefs B2) (image (apply_r sig) (occurs_free_fun_map fm)) ->
     
     fun_map_inv k (name_in_fundefs B1 :|: S) (add_fundefs B1 fm) (def_funs B1 B1 rho1 rho1) (def_funs B2 B2 rho2 rho2) i
                 (set_list (combine (all_fun_name B1) (all_fun_name B2)) sig).
   Proof.
     revert S fm rho1 rho2 i sig B1 B2. induction k as [k IHk] using lt_wf_rec1.
-    intros S fm rho1 rho2 i sig B1 B2 Hf Hrel Hun Hsub Hdis Hdis'' Hdis'.
+    intros S fm rho1 rho2 i sig B1 B2 Hf Hrel Hun Hsub Hdis Hdis'.
     intros f ft xs e rhoc B' f' HSin Heq1 Heq2.
     destruct (Decidable_name_in_fundefs B1) as [Dec]. destruct (Dec f).
     - rewrite def_funs_eq in Heq2; eauto. inv Heq2.
@@ -947,45 +1028,67 @@ Section Inline_correct.
         eapply Included_trans; [| eapply fun_in_fundefs_bound_var_fundefs; eauto ]. now sets.         
       + destruct k; eauto. rewrite <- fun_map_inv_eq. eapply fun_map_inv_antimon. eapply IHk.
         omega. eapply fun_map_inv_mon. eassumption. omega. eassumption. eassumption.
-        eassumption. now sets. now sets. now sets. eapply Setminus_Included_Included_Union. 
+        eassumption. now sets. now sets. eapply Setminus_Included_Included_Union. 
         eapply Included_trans. eapply occurs_free_in_fun. eapply find_def_correct. eassumption.
         sets.
     - rewrite def_funs_neq in Heq2; eauto.
       rewrite add_fundefs_not_in in Heq1; [| eassumption ]. inv HSin. contradiction.
       edestruct Hf. eassumption. eassumption. eassumption. destructAll. split; eauto. split; eauto.
       split; [| split; [| split; [| split ]]]; eauto.
-      + eapply preord_env_P_inj_def_funs_neq_r.
-        rewrite apply_r_set_list_f_eq. eapply preord_env_P_inj_extend_lst_not_In_P_r.
+      + eapply preord_env_P_inj_def_funs_neq_r_alt.
+        rewrite apply_r_set_list_f_eq. eapply preord_env_P_inj_extend_lst_not_In_P_r_alt.
         eassumption.
         * rewrite <- Same_set_all_fun_name.
-          eapply Disjoint_Included; [| | eapply Hdis'' ]. eapply Included_trans. eapply occurs_free_fun_map_get. eassumption.
-          now sets.
-          eapply Included_Setminus. eapply name_in_fundefs_funname_in_fundefs_Disjoint. eassumption.
-          eapply name_in_fundefs_bound_var_fundefs.
-        * rewrite apply_r_set_list_f_eq. eapply Disjoint_Included_l.
+          eapply Disjoint_Included; [| | eapply Hdis ]. eapply Dom_map_sub_map. eassumption.
+          eapply name_in_fundefs_bound_var_fundefs.           
+        * rewrite apply_r_set_list_f_eq. eapply Disjoint_Included_l. 
           intros x Hc. destruct Hc. destructAll.
           rewrite extend_lst_gso. eapply In_image. eassumption.
-          rewrite <- Same_set_all_fun_name. intros Hc. eapply Hdis''. constructor.
-          constructor. 
-          eapply name_in_fundefs_bound_var_fundefs. eassumption. intros Hc'.
-          eapply name_in_fundefs_funname_in_fundefs_Disjoint. eassumption. constructor; eauto.
-          eapply occurs_free_fun_map_get. eassumption. eassumption.
-          eapply Disjoint_sym. eapply Disjoint_Included; [| | eapply Hdis' ]. eapply image_monotonic.
-           eapply occurs_free_fun_map_get. eassumption. reflexivity. 
+          rewrite <- Same_set_all_fun_name. intros Hc. eapply Hdis. constructor.
+          eapply name_in_fundefs_bound_var_fundefs. eassumption. eapply Dom_map_sub_map; eassumption.
+          eapply Disjoint_Included_l. apply image_monotonic. eapply Dom_map_sub_map. eassumption.
+          sets.
       + eapply sub_map_trans. eassumption. eapply sub_map_def_funs.
         eapply Disjoint_Included; [| | eapply Hdis ]; sets. eapply name_in_fundefs_bound_var_fundefs. 
       + destruct k; eauto. rewrite <- fun_map_inv_eq in *.
         eapply fun_map_inv_add_fundefs_Disjoint; try eassumption.
-        rewrite Union_commut. rewrite Union_assoc. eapply Union_Disjoint_r.
-        * eapply Disjoint_Included; [| | eapply Hdis'' ].
-          eapply Union_Included. now sets.
-          eapply occurs_free_fun_map_get. eassumption.
-          eapply Included_Setminus.
-          eapply name_in_fundefs_funname_in_fundefs_Disjoint. eassumption. eapply name_in_fundefs_bound_var_fundefs. 
-        * eapply Disjoint_Included_r. eapply Dom_map_sub_map. eassumption.
-          eapply Disjoint_Included; [| | eapply Hdis ]. sets. eapply name_in_fundefs_bound_var_fundefs. 
+        * eapply Disjoint_Included; [| | eapply Hdis ]. eapply Dom_map_sub_map. eassumption.
+          eapply name_in_fundefs_bound_var_fundefs.
+        * eapply Disjoint_Included; [| | eapply Hdis' ]. eapply image_monotonic. eapply Dom_map_sub_map. eassumption.
+          reflexivity.
   Qed.
 
+  Lemma fun_in_fundefs_funname_in_exp f ft xs e B :
+    (f, ft, xs, e) \infun_in_fundefs B ->
+    funname_in_exp e \subset funname_in_fundefs B.
+  Proof.
+    induction B; intros Hin; inv Hin.
+    + inv H. sets.
+    + simpl. eapply Included_Union_preserv_r. eauto.
+  Qed.
+  
+  Definition funname_fun_map (fm : fun_map) : Ensemble var :=
+    fun x => exists f ft xs e, fm ! f = Some (ft, xs, e) /\ x \in funname_in_exp e.
+
+  Lemma funname_fun_map_fun_map_get f ft xs e (fm : fun_map) :
+    M.get f fm = Some (ft, xs, e) ->
+    funname_in_exp e \subset funname_fun_map fm.
+  Proof.
+    intros Hget z Hin. do 4 eexists. split; eauto.
+  Qed.
+  
+
+  Lemma funname_fun_map_add_fundefs B fm :
+    funname_fun_map (add_fundefs B fm) \subset (funname_in_fundefs B) :|: funname_fun_map fm.
+  Proof.
+    intros x [z Hin]. destructAll. destruct (Decidable_name_in_fundefs B). destruct (Dec z).
+    - edestruct name_in_fundefs_find_def_is_Some. eassumption. destructAll.
+      erewrite add_fundefs_in in H; [| eassumption ]. inv H.
+      left. eapply fun_in_fundefs_funname_in_exp. eapply find_def_correct. eassumption. eassumption.
+    - right. rewrite add_fundefs_not_in in H. do 4 eexists; split; eauto.
+      eassumption.
+  Qed.
+  
 
   Definition fun_map_vars (fm : fun_map) (F : Ensemble var) (sig : subst) :=
     forall f ft xs e,
@@ -993,11 +1096,11 @@ Section Inline_correct.
       unique_bindings e /\
       NoDup xs /\
       Disjoint _ (bound_var e) (FromList xs :|: occurs_free e) /\
-      Disjoint _ (bound_var e \\ funname_in_exp e) (occurs_free_fun_map fm :|: Dom_map fm) /\
-      Disjoint _ (FromList xs) (Dom_map fm :|: occurs_free_fun_map fm) /\
-      (* Disjoint _ (funname_in_exp e :|: funfv_in_exp e) (bound_var_fun_map fm) /\ *)
-
-      Disjoint _ F (bound_var e :|: image (apply_r sig) (occurs_free e \\ FromList xs :|: occurs_free_fun_map fm)).
+      Disjoint _ (bound_var e \\ funname_in_exp e) (Dom_map fm :|: funname_fun_map fm) /\
+      Disjoint _ (FromList xs) (Dom_map fm) /\
+      Disjoint _ (funname_in_exp e) (bound_var_fun_map fm) /\
+      
+      Disjoint _ F (bound_var e :|: image (apply_r sig) (occurs_free e \\ FromList xs)).
 
   Lemma fun_map_vars_set fm F sig x v :
     fun_map_vars fm F sig ->
@@ -1032,23 +1135,26 @@ Section Inline_correct.
       eapply name_in_fundefs_bound_var_fundefs. eassumption.
     - constructor.
   Qed.
-    
+
+
+  
+
+  
   Lemma fun_map_vars_def_funs fm S sig B xs :
     fun_map_vars fm S sig ->
     unique_bindings_fundefs B ->
 
     Disjoint _ (bound_var_fundefs B) (occurs_free_fundefs B) ->
-    Disjoint _ (bound_var_fundefs B \\ funname_in_fundefs B \\ name_in_fundefs B) (Dom_map fm :|: occurs_free_fun_map fm) ->
+    Disjoint _ (bound_var_fundefs B \\ funname_in_fundefs B \\ name_in_fundefs B) (Dom_map fm :|: funname_fun_map fm) ->
+    Disjoint _ (S \\ FromList xs) (bound_var_fundefs B :|: image (apply_r sig) (occurs_free_fundefs B)) ->    
     Disjoint _ (name_in_fundefs B) (bound_var_fun_map fm) ->
-    Disjoint _ (occurs_free_fundefs B) (bound_var_fun_map fm) ->
-    Disjoint _ (S \\ FromList xs) (bound_var_fundefs B :|: image (apply_r sig) (occurs_free_fundefs B :|: occurs_free_fun_map fm)) ->
-    (* Disjoint _ (funname_in_fundefs B :|: funfv_in_fundefs B) (bound_var_fun_map fm) -> *)
+    Disjoint _ (funname_in_fundefs B) (bound_var_fun_map fm) ->
     
     Datatypes.length (all_fun_name B) = Datatypes.length xs ->
     
     fun_map_vars (add_fundefs B fm) (S \\ FromList xs) (set_list (combine (all_fun_name B) xs) sig).
   Proof.
-    intros Hfm Hun Hdis1 Hdis (* Hdis' Hdis'' *) _ _ Hdis''' (* Hdis2 *) Hlen x ft ys e Hget. destruct (Decidable_name_in_fundefs B). destruct (Dec x).
+    intros Hfm Hun Hdis1 Hdis2 Hdis3 Hdis4 Hdis5 Hlen x ft ys e Hget. destruct (Decidable_name_in_fundefs B). destruct (Dec x).
     - edestruct name_in_fundefs_find_def_is_Some; eauto. destructAll. erewrite add_fundefs_in in Hget; eauto.
       inv Hget. edestruct unique_bindings_fun_in_fundefs. eapply find_def_correct. eassumption. eassumption. destructAll.
       assert (Hin1 : bound_var e \subset bound_var_fundefs B).
@@ -1056,92 +1162,53 @@ Section Inline_correct.
       assert (Hin2 : FromList ys \subset bound_var_fundefs B).
       { eapply Included_trans; [| eapply fun_in_fundefs_bound_var_fundefs; eapply find_def_correct; eauto ]. now sets. }
       
-      split. eauto. split. eauto. split; [| split; [| split; [| split ]]].
+      split. now eauto. split. now eauto. split; [| split; [| split; [| split ]]].
       + eapply Union_Disjoint_r. now sets.
         eapply fun_in_fundefs_Disjoint_bound_Var_occurs_free. eapply find_def_correct. eassumption.
         eassumption. now sets.
-      + eapply Union_Disjoint_r.
-        * eapply Disjoint_Included_r. eapply occurs_free_fun_map_add_fundefs.
-          eapply Union_Disjoint_r. eapply Union_Disjoint_r. 
-          eapply Disjoint_Included; [| | eapply Hdis1 ]; now sets. now sets.
-          eapply Disjoint_Included; [| | eapply Hdis ]. now sets.
+      + rewrite Dom_map_add_fundefs. eapply Union_Disjoint_r. eapply Union_Disjoint_r. now sets.
+        * eapply Disjoint_Included; [| | eapply Hdis2 ]. now sets.
           eapply Included_Setminus. now sets. 
           eapply fun_in_fundefs_bound_var_Setminus. eapply find_def_correct. eassumption. eassumption.
-        * rewrite Dom_map_add_fundefs. eapply Union_Disjoint_r. now sets.
-          eapply Disjoint_Included; [| | eapply Hdis ]. now sets.
-          eapply Included_Setminus. now sets. 
-          eapply fun_in_fundefs_bound_var_Setminus. eapply find_def_correct. eassumption. eassumption.
-      + eapply Union_Disjoint_r.
-        * rewrite Dom_map_add_fundefs. eapply Union_Disjoint_r. eassumption.
-          eapply Disjoint_Included_l.
-          eapply Included_Setminus. eassumption. 
-          eapply fun_in_fundefs_FromList_subset. eapply find_def_correct. eassumption. eassumption.
-          now sets.
-        * eapply Disjoint_Included_r. eapply occurs_free_fun_map_add_fundefs.
-          eapply Union_Disjoint_r. eapply Union_Disjoint_r.
-          eapply Disjoint_Included_l. eassumption. sets.
-          eassumption.
-          eapply Disjoint_Included_l. eapply Included_Setminus. eassumption. 
-          eapply fun_in_fundefs_FromList_subset. eapply find_def_correct. eassumption. eassumption.
-          sets.
-      (* + eapply Disjoint_Included_r. eapply bound_var_fun_map_add_fundefs_un. eassumption. *)
-      (*   eapply Union_Disjoint_r. *)
-      (*   * eapply Disjoint_Included_l. admit. admit. *)
-      (*     (* eapply fun_in_fundefs_bound_var_Setminus. *) *)
-      (*     (* (* now sets. admit. *)           *) *)
-      (*   * eapply Disjoint_Included; [| | eapply Hdis2 ]. now sets. admit. *)
-      (* (* eapply fun_in_fundefs_bound_var_Setminus. funname_in_fundefs_subset.  *) *)
+        * eapply Disjoint_Included_r. eapply funname_fun_map_add_fundefs. eapply Union_Disjoint_r.
+          ++ eapply Disjoint_Included_l. eapply fun_in_fundefs_bound_var_Setminus. eapply find_def_correct. eassumption.
+             eassumption. now sets.
+          ++ eapply Disjoint_Included_l. eapply fun_in_fundefs_bound_var_Setminus'. eapply find_def_correct. eassumption.
+             eassumption. now sets.
+      + rewrite Dom_map_add_fundefs. eapply Union_Disjoint_r. eassumption.
+        eapply Disjoint_Included_l.
+        eapply Included_Setminus. eassumption. 
+        eapply fun_in_fundefs_FromList_subset. eapply find_def_correct. eassumption. eassumption.
+        now sets.
+      + eapply Disjoint_Included_r. eapply bound_var_fun_map_add_fundefs_un. eassumption.
+        eapply Disjoint_Included_l. eapply fun_in_fundefs_funname_in_exp. eapply find_def_correct. eassumption.
+        eapply Union_Disjoint_r. now sets. eassumption.
       + eapply Union_Disjoint_r. now sets. eapply Disjoint_Included_r.
         eapply image_apply_r_set_list. now eauto. eapply Union_Disjoint_r. now sets.
-        rewrite <- Same_set_all_fun_name. rewrite Setminus_Union_distr.
-        eapply Disjoint_Included_r. eapply image_monotonic. eapply Included_Union_compat. reflexivity.
-        eapply Included_Setminus_compat. eapply occurs_free_fun_map_add_fundefs. reflexivity.
-        rewrite !Setminus_Union_distr. rewrite Setminus_Same_set_Empty_set. repeat normalize_sets.
-        rewrite image_Union. eapply Union_Disjoint_r; [| now xsets ].
-        eapply Disjoint_Included_r. eapply image_monotonic.
-        eapply Included_Setminus_compat. eapply Included_Setminus_compat.
-        eapply occurs_free_in_fun. eapply find_def_correct. eassumption. reflexivity. reflexivity.
-        rewrite !Setminus_Union_distr. rewrite Setminus_Same_set_Empty_set.
-        rewrite Setminus_Union. rewrite (Setminus_Included_Empty_set (name_in_fundefs _)); [| now sets ].
-        repeat normalize_sets. xsets.
+        rewrite <- Same_set_all_fun_name.
+        eapply Disjoint_Included; [| | eapply Hdis3 ].
+        eapply Included_Union_preserv_r. eapply image_monotonic. do 2 eapply Setminus_Included_Included_Union.
+        eapply Included_trans. eapply occurs_free_in_fun. eapply find_def_correct. eassumption. now sets. reflexivity.
     - rewrite add_fundefs_not_in in Hget; eauto. edestruct Hfm. eassumption. destructAll.
       split; eauto. split; eauto. split; [| split; [| split; [| split ]]].
       + now sets.        
-      + rewrite Dom_map_add_fundefs. eapply Union_Disjoint_r.
-        * eapply Disjoint_Included_r. eapply occurs_free_fun_map_add_fundefs. eapply Union_Disjoint_r; [| now sets ].
-          (* eapply Union_Disjoint_r. *)
-          (* eapply Disjoint_sym. eapply Disjoint_Included_r; [| eassumption ]. *)
-          (* eapply Included_trans; [| eapply bound_var_fun_map_get; eauto ]. now sets. *)
-          (* eapply Disjoint_sym. eapply Disjoint_Included_r; [| eassumption ]. *)
-        (* eapply Included_trans; [| eapply bound_var_fun_map_get; eauto ]. now sets. *) 
-          eapply Union_Disjoint_r.  admit. admit.
-        * eapply Union_Disjoint_r. sets.
-          admit.
-          (* eapply Disjoint_sym. eapply Disjoint_Included_r; [| eassumption ]. *)
-          (* eapply Included_trans; [| eapply bound_var_fun_map_get; eauto ]. now sets. *)
-          now sets.
-      + rewrite Dom_map_add_fundefs. eapply Union_Disjoint_r. eapply Union_Disjoint_r.
-        admit. 
-        (* eapply Disjoint_sym. eapply Disjoint_Included_r; [| eassumption ]. *)
-        (* eapply Included_trans; [| eapply bound_var_fun_map_get; eauto ]. now sets. *)
-        now sets.
-        eapply Disjoint_Included_r. eapply occurs_free_fun_map_add_fundefs. 
-        eapply Union_Disjoint_r; [| now sets ]. eapply Union_Disjoint_r.
+      + rewrite Dom_map_add_fundefs. eapply Union_Disjoint_r. eapply Union_Disjoint_r. 
+        * eapply Disjoint_sym. eapply Disjoint_Included_r; [| eassumption ].
+          eapply Included_trans; [| eapply bound_var_fun_map_get; eauto ]. now sets.
+        * sets.
+        * eapply Disjoint_Included_r. eapply funname_fun_map_add_fundefs. eapply Union_Disjoint_r; [| now sets ].
+          eapply Disjoint_sym. eapply Disjoint_Included_r; [| eassumption ].
+          eapply Included_trans; [| eapply bound_var_fun_map_get; eauto ]. now sets.         
+      + rewrite Dom_map_add_fundefs. eapply Union_Disjoint_r; [| now sets ].
         eapply Disjoint_sym. eapply Disjoint_Included_r; [| eassumption ].
         eapply Included_trans; [| eapply bound_var_fun_map_get; eauto ]. now sets.
-        eapply Disjoint_sym. eapply Disjoint_Included_r; [| eassumption ].
-        eapply Included_trans; [| eapply bound_var_fun_map_get; eauto ]. now sets.
-      (* + eapply Disjoint_Included_r. eapply bound_var_fun_map_add_fundefs_un. eassumption. *)
-      (*   eapply Union_Disjoint_r; [| eassumption ]. admit. *)
+      + eapply Disjoint_Included_r. eapply bound_var_fun_map_add_fundefs_un. eassumption.
+        eapply Union_Disjoint_r; [| eassumption ].
+        * eapply Disjoint_sym. eapply Disjoint_Included_r. eapply funname_fun_map_fun_map_get. eassumption.
+          sets.
       + eapply Union_Disjoint_r. now sets. 
         eapply Disjoint_Included_r. eapply image_apply_r_set_list. eassumption.
-        eapply Union_Disjoint_r. now sets. eapply Disjoint_Included_r.
-        rewrite <- Same_set_all_fun_name. rewrite Setminus_Union_distr. eapply image_monotonic.
-        eapply Included_Union_compat. reflexivity. eapply Included_Setminus_compat.
-        eapply occurs_free_fun_map_add_fundefs. reflexivity.
-        rewrite !Setminus_Union_distr. rewrite Setminus_Same_set_Empty_set. repeat normalize_sets.
-        rewrite !image_Union in *. eapply Union_Disjoint_r. now xsets. eapply Union_Disjoint_r; [| now xsets ]. 
-        xsets.
+        eapply Union_Disjoint_r. now sets. xsets.
   Qed.
   
   Opaque preord_exp'.
@@ -1150,9 +1217,9 @@ Section Inline_correct.
     (forall e sig fm st S
             (Hun : unique_bindings e)
             (Hdis1 : Disjoint _ (bound_var e) (occurs_free e))
-            (Hdis2 : Disjoint _ S (bound_var e :|: image (apply_r sig) (occurs_free e :|: occurs_free_fun_map fm)))
-            (Hdis3 : Disjoint _ (bound_var e \\ funname_in_exp e) (Dom_map fm :|: occurs_free_fun_map fm))
-            (* (Hdis4 : Disjoint _ (funname_in_exp e :|: funfv_in_exp e) (bound_var_fun_map fm)) *)
+            (Hdis2 : Disjoint _ S (bound_var e :|: image (apply_r sig) (occurs_free e)))
+            (Hdis3 : Disjoint _ (bound_var e \\ funname_in_exp e) (Dom_map fm :|: funname_fun_map fm))
+            (Hdis4 : Disjoint _ (funname_in_exp e) (bound_var_fun_map fm))
             
             (Hfm : fun_map_vars fm S sig),
         {{ fun _ s => fresh S (next_var (fst s)) }}
@@ -1165,15 +1232,16 @@ Section Inline_correct.
              (forall k rho1 rho2,
                  preord_env_P_inj cenv PG (occurs_free e) k (apply_r sig) rho1 rho2 ->
                  Disjoint _ (bound_var e) (Dom_map rho1) ->
+                 Disjoint _ S (image (apply_r sig) (Dom_map rho1)) ->
                  fun_map_inv d (occurs_free e) fm rho1 rho2 k sig ->
                  preord_exp cenv P1 PG k (e, rho1) (e', rho2)) }} ) /\ 
 
     (forall B sig sig0 fm st S
             (Hun : unique_bindings_fundefs B)
             (Hdis1 : Disjoint _ (bound_var_fundefs B) (occurs_free_fundefs B))
-            (Hdis2 : Disjoint _ S (bound_var_fundefs B :|: image (apply_r sig) (occurs_free_fundefs B :|: occurs_free_fun_map fm)))
-            (Hdis3 : Disjoint _ (bound_var_fundefs B \\ name_in_fundefs B \\ funname_in_fundefs B) (Dom_map fm :|: occurs_free_fun_map fm))
-            (* (Hdis4 : Disjoint _ (funname_in_fundefs B :|: funfv_in_fundefs B) (bound_var_fun_map fm)) *)
+            (Hdis2 : Disjoint _ S (bound_var_fundefs B :|: image (apply_r sig) (occurs_free_fundefs B :|: name_in_fundefs B)))
+            (Hdis3 : Disjoint _ (bound_var_fundefs B \\ name_in_fundefs B \\ funname_in_fundefs B) (Dom_map fm :|: funname_fun_map fm))
+            (Hdis4 : Disjoint _ (funname_in_fundefs B) (bound_var_fun_map fm))
             
             (Hfm : fun_map_vars fm S sig), 
         {{ fun _ s => fresh S (next_var (fst s)) }}
@@ -1182,7 +1250,7 @@ Section Inline_correct.
              fresh S (next_var (fst s')) /\ next_var (fst s) <= next_var (fst s') /\
              unique_bindings_fundefs B' /\
              occurs_free_fundefs B' \subset image (apply_r sig) (occurs_free_fundefs B :|: occurs_free_fun_map fm) /\
-             bound_var_fundefs B' \subset (Range (next_var (fst s)) (next_var (fst s'))) /\
+             bound_var_fundefs B' \\ name_in_fundefs B' \subset (Range (next_var (fst s)) (next_var (fst s'))) /\
              all_fun_name B' = apply_r_list sig (all_fun_name B) /\
              (forall f xs ft e1,
                  find_def f B = Some (ft, xs, e1) ->
@@ -1190,9 +1258,11 @@ Section Inline_correct.
                    find_def (apply_r sig f) B' = Some (ft, xs', e2) /\
                    length xs = length xs' /\ NoDup xs' /\ FromList xs' \subset S /\
                    (forall rho1 rho2 k,
-                       preord_env_P_inj cenv PG (occurs_free_fundefs B) k (apply_r sig <{ xs ~> xs' }>) rho1 rho2 ->
+                       preord_env_P_inj cenv PG (occurs_free_fundefs B :|: name_in_fundefs B :|: FromList xs)
+                                        k (apply_r sig <{ xs ~> xs' }>) rho1 rho2 ->
                        Disjoint _ (bound_var e1) (Dom_map rho1) ->
-                       fun_map_inv d (occurs_free_fundefs B) fm rho1 rho2 k sig ->
+                       Disjoint _ (S \\ FromList xs') (image (apply_r sig <{ xs ~> xs' }>) (Dom_map rho1)) ->
+                       fun_map_inv d (occurs_free_fundefs B :|: name_in_fundefs B :|: FromList xs) fm rho1 rho2 k (set_list (combine xs xs') sig) ->
                        preord_exp cenv P1 PG k (e1, rho1) (e2, rho2))) }}).
 
   Proof.
@@ -1213,10 +1283,9 @@ Section Inline_correct.
         repeat normalize_bound_var_in_ctx. repeat normalize_occurs_free_in_ctx.
         eapply Union_Disjoint_r. now sets.
         eapply Union_Disjoint_r. now sets.
-        eapply Disjoint_Included; [| | eapply Hdis2 ].
-        rewrite Setminus_Union_distr. rewrite !image_Union. now xsets. now sets.
+        eapply Disjoint_Included; [| | eapply Hdis2 ]; sets.
       + eapply Disjoint_Included_l; [| eassumption ]. normalize_bound_var. sets.
-      (* + eassumption. *)
+      + eassumption.
       + eapply fun_map_vars_set. eassumption.
       + intros e' w2. eapply return_triple.
         intros _ st'. intros [Hf1 [Hf2 [Hf3 [Hf4 [Hun [Hsub [Hsub' Hsem]]]]]]].
@@ -1236,7 +1305,7 @@ Section Inline_correct.
           eapply Range_Subset. zify; omega. reflexivity.
           eapply Included_trans. eapply Singleton_Included. eassumption. eapply Range_Subset. reflexivity.
           zify; omega.
-        * intros r1 r2 k Henv Hdis Hfm'. eapply preord_exp_const_compat.
+        * intros r1 r2 k Henv Hdis Hdis' Hfm'. eapply preord_exp_const_compat.
           eassumption. eassumption.
           eapply Forall2_preord_var_env_map. eassumption. normalize_occurs_free. now sets.          
           intros. eapply Hsem. 
@@ -1246,31 +1315,22 @@ Section Inline_correct.
           -- rewrite preord_val_eq. split. reflexivity.
              eapply Forall2_Forall2_asym_included. eassumption.
           -- intros Hc. eapply Hdis2. constructor. eapply Hf. eapply Hf1. 
-             right. normalize_occurs_free. rewrite !image_Union. left. right. eassumption.
+             right. normalize_occurs_free. rewrite !image_Union. right. eassumption.
           -- repeat normalize_bound_var_in_ctx. rewrite Dom_map_set.
              eapply Union_Disjoint_r.
              ++ eapply Disjoint_Singleton_r. eassumption.
-               (* eapply Disjoint_Included_r. eapply occurs_free_in_env_set. simpl. normalize_sets. *)
-               (*  eapply Disjoint_Included; [| | eapply Hdis]; sets. *)
              ++ sets.
-                (* eapply Union_Disjoint_r. *)
-                (* ** eapply Disjoint_Singleton_r. eassumption. *)
-                (* ** eapply Disjoint_Included; [| | eapply Hdis]; sets. *)
-            (* eapply Disjoint_Included_r. *)
-            (*  eapply Included_trans. eapply image_monotonic. eapply occurs_free_in_env_set. simpl. repeat normalize_sets. *)
-            (*  now eapply image_apply_r_set. *)
-            (*  eapply Union_Disjoint_r. now sets. sets.  *)
+          -- eapply Disjoint_Included_r. rewrite Dom_map_set. eapply image_apply_r_set.
+             rewrite Setminus_Union_distr. rewrite Setminus_Same_set_Empty_set. normalize_sets.
+             eapply Union_Disjoint_r. now sets. now sets. 
           -- eapply fun_map_inv_antimon. eapply fun_map_inv_set. eapply fun_map_inv_i_mon. eassumption. omega.
              intros Hc. inv Hc. inv H2.
-             ++ eapply Hdis. normalize_bound_var. constructor. now right. eassumption.
+             ++ eapply Hdis. normalize_bound_var. constructor. now right. eexists; eauto.
              ++ eapply Hdis3. constructor. normalize_bound_var. simpl. constructor. now right.
                 intros Hc. eapply H1. eapply funname_in_exp_subset. eassumption.
                 now left; eauto.
-             ++ eapply Hdis3. normalize_bound_var. constructor. constructor. now right. simpl.
-                intros Hc. eapply H1. eapply funname_in_exp_subset. eassumption.
-                now right; eauto.
-             ++ intros Hc. eapply Hdis2. constructor; try eassumption.
-                eapply fresh_Range; [| eassumption ]. eassumption. rewrite image_Union. eauto.
+             ++ intros Hc. eapply Hdis'. constructor; try eassumption.
+                eapply fresh_Range; [| eassumption ]. eassumption.
              ++ normalize_occurs_free. rewrite !Union_assoc. rewrite Union_Setminus_Included; sets; tci.
     - (* Ecase [] *)
       admit.
@@ -1284,17 +1344,27 @@ Section Inline_correct.
       simpl. destruct (update_funDef St IH f2 sig st). 
       eapply bind_triple. eapply pre_transfer_r. now eapply get_names_lst_fresh. intros xs w. simpl.
       eapply pre_curry_l. intros Hf. eapply pre_curry_l. intros Hnd.  eapply pre_curry_l. intros Hlen.
+
+      assert (Hsame1 : bound_var_fundefs f2 \\ funname_in_fundefs f2 \\ name_in_fundefs f2 \subset bound_var (Efun f2 e) \\ funname_in_exp (Efun f2 e)).
+      { normalize_bound_var. simpl. rewrite !Setminus_Union_distr. eapply Included_Union_preserv_l.
+        rewrite <- !Setminus_Union. eapply Included_Setminus; [| now sets ].
+        eapply Disjoint_Included_r. eapply funname_in_exp_subset. sets. } 
+
+      assert (Hsame2 : bound_var e \\ funname_in_exp e \subset bound_var (Efun f2 e) \\ funname_in_exp (Efun f2 e)).
+      { normalize_bound_var. simpl. rewrite !Setminus_Union_distr. eapply Included_Union_preserv_r.
+        rewrite (Union_commut _ (funname_in_exp _)). rewrite <- Setminus_Union. eapply Included_Setminus; [| now sets ].
+        eapply Disjoint_Included_r. eapply Union_Included. eapply funname_in_fundefs_subset.
+        eapply name_in_fundefs_bound_var_fundefs. sets. } 
+
       
       assert (Hfm' : fun_map_vars (add_fundefs f2 fm) (S \\ FromList xs) (set_list (combine (all_fun_name f2) xs) sig)).
       { eapply fun_map_vars_def_funs; (try now eauto).
         + repeat normalize_bound_var_in_ctx. repeat normalize_occurs_free_in_ctx.
           eapply Disjoint_Included; [| | eapply Hdis1 ]; sets.
-        + eapply Disjoint_Included_l; [| eapply Hdis3 ]. simpl. admit.
-        + admit. (* Disjoint var (name_in_fundefs f2) (bound_var_fun_map fm) *)
-        + admit.
-        (* + eapply Disjoint_Included_l; [| eassumption ]. simpl. sets. *)
-        + repeat normalize_bound_var_in_ctx. repeat normalize_occurs_free_in_ctx.
-          eapply Disjoint_Included; [| | eapply Hdis2 ]; sets. }      
+        + eapply Disjoint_Included_l; [| eapply Hdis3 ]. eassumption.
+        + repeat normalize_bound_var_in_ctx. repeat normalize_occurs_free_in_ctx. xsets.
+        + sets.
+        + sets. }
       
       eapply bind_triple. 
       { do 2 eapply frame_rule. eapply IHB with (S := S \\ FromList xs).
@@ -1305,21 +1375,18 @@ Section Inline_correct.
           rewrite image_Union in Hdis2. eapply Union_Disjoint_r. now sets.
           eapply Disjoint_Included_r. eapply image_apply_r_set_list. now eauto.
           eapply Union_Disjoint_r. now sets.
-          rewrite <- Same_set_all_fun_name. rewrite Setminus_Union_distr. rewrite image_Union. eapply Union_Disjoint_r.
-          now xsets.
-          eapply Disjoint_Included_r. eapply image_monotonic. eapply Included_Setminus_compat. eapply occurs_free_fun_map_add_fundefs. reflexivity.
-          rewrite !Setminus_Union_distr. rewrite Setminus_Same_set_Empty_set. repeat normalize_sets. rewrite image_Union. xsets.
+          rewrite <- Same_set_all_fun_name. xsets. 
         - repeat normalize_occurs_free_in_ctx. repeat normalize_bound_var_in_ctx.
           rewrite Dom_map_add_fundefs. eapply Union_Disjoint_r.
           + eapply Union_Disjoint_r. now sets.
-            eapply Disjoint_Included; [| | eapply Hdis3 ]. now sets. admit.            
-          + eapply Disjoint_Included_r. eapply occurs_free_fun_map_add_fundefs. eapply Union_Disjoint_r.
-            eapply Union_Disjoint_r. eapply Disjoint_Included; [| | eapply Hdis1 ]. now sets. now sets.
-            now sets.
-            eapply Disjoint_Included; [| | eapply Hdis3 ]. now sets. admit.
+            eapply Disjoint_Included; [| | eapply Hdis3 ]. now sets.
+            rewrite Setminus_Union. rewrite Union_commut. rewrite <- Setminus_Union. eassumption.
+          + eapply Disjoint_Included_r. eapply funname_fun_map_add_fundefs. eapply Union_Disjoint_r. now sets.
+            eapply Disjoint_Included; [| | eapply Hdis3 ]. now sets.
+            rewrite Setminus_Union. rewrite Union_commut. rewrite <- Setminus_Union. eassumption.
         - eapply Disjoint_Included_r. eapply bound_var_fun_map_add_fundefs_un. eassumption. eapply Union_Disjoint_r.
-          + eapply Union_Disjoint_l. now sets. admit. (* ?? *)
-          + eapply Disjoint_Included_l; [| eassumption ]. sets.
+          + now sets.
+          + now sets.
         - eassumption. }
 
       intros fds' w'. simpl.
@@ -1336,42 +1403,44 @@ Section Inline_correct.
               eapply Union_Disjoint_r. now sets. eapply Disjoint_Included_r.
               eapply image_apply_r_set_list. now eauto.
               rewrite image_Union in Hdis2. eapply Union_Disjoint_r. now xsets.
-              rewrite <- Same_set_all_fun_name. rewrite Setminus_Union_distr. rewrite image_Union.
-              eapply Union_Disjoint_r. now xsets.
-              eapply Disjoint_Included_r. eapply image_monotonic. eapply Included_Setminus_compat. eapply occurs_free_fun_map_add_fundefs. reflexivity.
-              rewrite !Setminus_Union_distr. rewrite image_Union. xsets.
+              rewrite <- Same_set_all_fun_name. sets.
             + repeat normalize_bound_var_in_ctx. repeat normalize_occurs_free_in_ctx.
               rewrite Dom_map_add_fundefs. eapply Union_Disjoint_r.
               * eapply Union_Disjoint_r.
                 -- eapply Disjoint_Included_r. eapply name_in_fundefs_bound_var_fundefs. now sets.
-                -- eapply Disjoint_Included; [| | eapply Hdis3 ]; sets. simpl. admit.
-              * eapply Disjoint_Included_r. eapply occurs_free_fun_map_add_fundefs.
-                eapply Union_Disjoint_r. eapply Union_Disjoint_r. 
-                -- eapply Disjoint_Included; [| | eapply Hdis1 ]; sets.
-                -- eapply Disjoint_Included_r. eapply name_in_fundefs_bound_var_fundefs. now sets.
-                -- eapply Disjoint_Included; [| | eapply Hdis3 ]. now sets.
-                   simpl. admit.
+                -- eapply Disjoint_Included; [| | eapply Hdis3 ]; sets.
+              * eapply Disjoint_Included_r. eapply funname_fun_map_add_fundefs. eapply Union_Disjoint_r.
+                -- eapply Disjoint_Included_r. eapply funname_in_fundefs_subset. sets.
+                -- eapply Disjoint_Included; [| | eapply Hdis3 ]. now sets. eassumption.
             + eapply Disjoint_Included_r. eapply bound_var_fun_map_add_fundefs_un. eassumption. eapply Union_Disjoint_r.
-              * admit. (* ?? *)
-              * eapply Disjoint_Included; [| | eapply Hdis4 ]. reflexivity. simpl. admit. 
-            + eassumption. }
-        
-      simpl. intros u w1 [Hyp Hyp']. split. eapply Hyp'. eassumption. }
-      intros e' w''. eapply return_triple. intros _ w''' Hyp. destructAll.
+              * eapply Disjoint_Included_l. eapply funname_in_exp_subset. sets.
+              * sets.
+            + eassumption. }        
+        simpl. intros u w1 [Hyp Hyp']. split. eapply Hyp'. eassumption. }
+
       assert (Hnd' := NoDup_all_fun_name _ H2).
+      assert (Hseq :  apply_r_list (set_list (combine (all_fun_name f2) xs) sig) (all_fun_name f2) = xs).
+      { rewrite apply_r_list_eq. reflexivity. now eauto. now eauto. }
+
+      intros e' w''. eapply return_triple. intros _ w''' Hyp. destructAll.
       split; [| split; [| split; [| split; [| split ]]]].
       * eapply fresh_monotonic; [| eassumption ]. sets.
       * zify; omega. 
       * constructor. eassumption. eassumption.
-        eapply Disjoint_Included. eassumption. eassumption.
-        eapply Disjoint_sym. eapply Disjoint_Range. reflexivity.
+        eapply Disjoint_Included_r. eapply Included_Union_Setminus with (s2 := name_in_fundefs fds'). now tci.
+        eapply Union_Disjoint_r.
+        -- eapply Disjoint_Included. eassumption. eassumption.
+           eapply Disjoint_sym. eapply Disjoint_Range. reflexivity.
+        -- rewrite Same_set_all_fun_name. rewrite H12. rewrite Hseq.
+           eapply Disjoint_Included. eassumption. eassumption.
+           eapply Disjoint_sym. eapply Disjoint_Range. zify; omega.
       * repeat normalize_occurs_free. eapply Union_Included.
         -- eapply Included_trans. eapply Included_Setminus. eapply Disjoint_sym.
            eapply occurs_free_fundefs_name_in_fundefs_Disjoint. reflexivity.
            eapply Setminus_Included_Included_Union. eapply Included_trans. eassumption.
            eapply Included_trans. eapply image_apply_r_set_list. now eauto.
            rewrite (Same_set_all_fun_name fds'). rewrite H12.
-           rewrite apply_r_list_eq; eauto. eapply Union_Included. now sets.
+           rewrite apply_r_list_eq; eauto. eapply Union_Included. now sets. 
            eapply Included_Union_preserv_l. rewrite <- Same_set_all_fun_name.
            rewrite Setminus_Union_distr. rewrite !image_Union. eapply Union_Included. now sets.
            eapply Included_trans. eapply image_monotonic. eapply Included_Setminus_compat.
@@ -1390,12 +1459,14 @@ Section Inline_correct.
            rewrite !Setminus_Union_distr, Setminus_Same_set_Empty_set. repeat normalize_sets.
            rewrite image_Union. now xsets.
       * normalize_bound_var. eapply Union_Included.
-        -- eapply Included_trans. eassumption. eapply Range_Subset. eassumption. zify; omega.
+        -- eapply Included_trans.
+           eapply Included_Union_Setminus with (s2 := name_in_fundefs fds'). now tci. eapply Union_Included.
+           ++ eapply Included_trans. eassumption. eapply Range_Subset; zify; omega. 
+           ++ rewrite Same_set_all_fun_name. rewrite H12. rewrite Hseq.
+              eapply Included_trans. eassumption. eapply Range_Subset; zify; omega. 
         -- eapply Included_trans. eassumption. eapply Range_Subset. zify; omega. reflexivity.
-      * intros k rho1 rho2 Henv Hdis Hfm''. eapply preord_exp_fun_compat.
+      * intros k rho1 rho2 Henv Hdis Hdis' Hfm''. eapply preord_exp_fun_compat.
         eassumption. eassumption.
-        assert (Hseq :  apply_r_list (set_list (combine (all_fun_name f2) xs) sig) (all_fun_name f2) = xs).
-        { rewrite apply_r_list_eq. reflexivity. now eauto. now eauto. }
         assert (Hrel : preord_env_P_inj cenv PG
                                         (name_in_fundefs f2 :|: occurs_free (Efun f2 e)) 
                                         (k - 1) (apply_r (set_list (combine (all_fun_name f2) xs) sig))
@@ -1408,10 +1479,10 @@ Section Inline_correct.
               rewrite H12. rewrite FromList_apply_list. eapply In_image.
               rewrite <- Same_set_all_fun_name. eassumption.
             + rewrite preord_val_eq. intros vs1 vs2 j t1 ys1 e2 rho1' Hlen' Hfind Hset.
-              edestruct H13. eassumption. destructAll.
+              edestruct H13. eassumption. destructAll. 
               edestruct set_lists_length2 with (xs2 := x0) (vs2 := vs2) (rho' := def_funs fds' fds' rho2 rho2). 
               now eauto. eassumption. now eauto. do 3 eexists. split. eassumption. split. now eauto. 
-              intros Hlt Hvs. eapply preord_exp_post_monotonic. eassumption. eapply H18.
+              intros Hlt Hvs. eapply preord_exp_post_monotonic. eassumption. eapply H18. 
               * eapply preord_env_P_inj_set_lists_alt; [| eassumption | | | | | now eauto | now eauto ]. 
                 -- eapply preord_env_P_inj_antimon. eapply IHi. eassumption. omega.
                    normalize_occurs_free. sets.
@@ -1429,24 +1500,46 @@ Section Inline_correct.
                 eapply Union_Disjoint_r. eapply unique_bindings_fun_in_fundefs. eapply find_def_correct. eassumption. eassumption.
                 eapply Disjoint_Included_l; [| eapply Hdis ]. normalize_bound_var. eapply Included_Union_preserv_l.
                 eapply Included_trans; [| eapply fun_in_fundefs_bound_var_fundefs ]; [| eapply find_def_correct; eassumption ]. sets.
+              * eapply Disjoint_Included_r. rewrite Dom_map_set_lists; eauto. rewrite Dom_map_def_funs.
+                eapply image_extend_lst_Included. eassumption. eapply Union_Disjoint_r; [| now sets ].
+                eapply Disjoint_Included_r. eapply image_apply_r_set_list. now auto. rewrite <- Same_set_all_fun_name.
+                rewrite !Setminus_Union_distr, Setminus_Same_set_Empty_set. repeat normalize_sets.
+                eapply Union_Disjoint_r. now sets.
+                rewrite (Setminus_Union _ (FromList ys1)). rewrite (Union_commut (FromList ys1)). rewrite <- Setminus_Union. 
+                rewrite Setminus_Same_set_Empty_set. repeat normalize_sets. xsets.
               * eapply fun_map_inv_antimon. eapply fun_map_inv_set_lists; [ | | | now eauto ].
                 eapply fun_map_inv_set_lists_r; [| | now eauto ]. 
-                -- rewrite <- Hseq. rewrite <- H12. eapply fun_map_inv_def_funs.
+                -- rewrite <- Hseq. rewrite <- H12. eapply fun_map_inv_sig_extend_Disjoint.
+                   eapply fun_map_inv_def_funs.
                    eapply fun_map_inv_i_mon. eassumption. omega. eapply preord_env_P_inj_antimon.
                    rewrite H12. rewrite Hseq. eapply IHi. eassumption. omega. normalize_occurs_free. sets.
                    eassumption. normalize_occurs_free. now sets.
                    repeat normalize_bound_var_in_ctx. now sets.
-                   eapply Disjoint_Included; [ | | eapply Hdis3 ]. now sets. simpl. admit.
-                   eapply Disjoint_Included_l. eapply Included_trans. eapply name_in_fundefs_bound_var_fundefs. eassumption.
-                   eapply Disjoint_Included; [| | eapply Hdis2 ]. rewrite image_Union. now sets.
-                   intros z Hin. eapply Hf. unfold Ensembles.In, Range in *. zify. omega.
-                -- eapply Disjoint_Included_l. eassumption. eapply Disjoint_Included_r.
-                   eapply image_apply_r_set_list. now eauto. eapply Union_Disjoint_r. now sets.
-                   eapply Disjoint_Included; [| | eapply Hdis2 ]. rewrite <- Same_set_all_fun_name.
-                   eapply Included_trans. eapply image_monotonic. eapply Included_Setminus_compat.
-                   eapply occurs_free_fun_map_add_fundefs. reflexivity. rewrite !Setminus_Union_distr.
-                   rewrite Setminus_Same_set_Empty_set. repeat normalize_sets. 
-                   normalize_occurs_free. rewrite !image_Union. now xsets. now sets.
+                   eapply Disjoint_Included; [ | | eapply Hdis' ]. now sets.
+                   rewrite Same_set_all_fun_name, H12, Hseq. 
+                   eapply Included_trans. eassumption. 
+                   intros z Hin. eapply Hf. unfold Range, Ensembles.In in Hin. zify. omega.
+
+                   rewrite Dom_map_def_funs. eapply Union_Disjoint_r.
+                   eapply unique_bindings_fun_in_fundefs. eapply find_def_correct. eassumption. eassumption.
+                   eapply Disjoint_Included_l; [| eassumption ].
+                   normalize_bound_var. eapply Included_Union_preserv_l.
+                   eapply Included_trans; [|  eapply fun_in_fundefs_bound_var_fundefs; eapply find_def_correct; eassumption ].
+                   now sets.
+                -- rewrite image_f_eq_subdomain.
+                   2:{ rewrite apply_r_set_list_f_eq. eapply f_eq_subdomain_extend_lst_Disjoint.
+                       rewrite Dom_map_def_funs. eapply Union_Disjoint_r.
+                       eapply unique_bindings_fun_in_fundefs. eapply find_def_correct. eassumption. eassumption.
+                       eapply Disjoint_Included_l; [| eassumption ]. normalize_bound_var. eapply Included_Union_preserv_l.
+                       eapply Included_trans; [|  eapply fun_in_fundefs_bound_var_fundefs; eapply find_def_correct; eassumption ].
+                       now sets. }
+                   eapply Disjoint_Included_l. eassumption.
+                   eapply Disjoint_Included_r. 
+                   eapply image_apply_r_set_list. now eauto. eapply Union_Disjoint_r. 
+                   now sets.
+                   eapply Disjoint_Included; [| | eapply Hdis' ]. rewrite <- Same_set_all_fun_name.
+                   rewrite Dom_map_def_funs. rewrite !Setminus_Union_distr. rewrite image_Union. eapply Union_Included.
+                   now sets. now sets. now sets.
                 -- eapply unique_bindings_fun_in_fundefs. eapply find_def_correct. eassumption. eassumption.
                 -- eapply Disjoint_Included_r. eapply Included_Union_compat.
                    eapply Dom_map_def_funs. eapply Dom_map_add_fundefs.
@@ -1457,19 +1550,14 @@ Section Inline_correct.
                    eapply Union_Disjoint_r. now sets.
                    eapply Disjoint_Included; [| | eapply Hdis3 ]. now sets.
                    eapply Included_trans. eapply fun_in_fundefs_FromList_subset. eapply find_def_correct. eassumption. eassumption.
-                   admit. 
-                   (* simpl. rewrite <-Setminus_Union.  *)
-                   (* eapply Included_trans. eapply fun_in_fundefs_FromList_subset. eapply find_def_correct. eassumption. eassumption. *)
-                   (* simpl. normalize_bound_var. *)
-                   (* eapply Disjoint_Included_l. eapply Included_trans; [| eapply fun_in_fundefs_bound_var_fundefs; eapply find_def_correct; eapply Hfind ]. *)
-                   (* now sets. eapply Disjoint_Included; [| | eapply Hdis3 ]. now sets. normalize_bound_var. now sets. *)
+                   eassumption. 
                 -- normalize_occurs_free. sets.
           - inv HIn. contradiction. rewrite def_funs_neq in Hgetx; [| eassumption ]. eapply Henv in Hgetx; [| eassumption ]. destructAll. 
             eexists. rewrite apply_r_set_list_f_eq. rewrite extend_lst_gso. rewrite def_funs_neq. 
             split; eauto. eapply preord_val_monotonic. eassumption. omega. 
-            + intros Hc. eapply Same_set_all_fun_name in Hc. rewrite H12 in Hc.
-              rewrite apply_r_list_eq in Hc; [| | now eauto ]. eapply Hdis2. constructor. 
-              2:{ right. eapply In_image. now left; eauto. } 
+            + intros Hc. eapply Same_set_all_fun_name in Hc. rewrite H12 in Hc. 
+              rewrite apply_r_list_eq in Hc; [| | now eauto ]. eapply Hdis2. constructor . 
+              2:{ right. eapply In_image. eauto. } 
               eapply fresh_Range. 2:{ eapply Hsub. eassumption. } eassumption. eassumption.
             + rewrite <- Same_set_all_fun_name. intros Hc. eapply Hdis1. constructor. normalize_bound_var. left.
               now eapply name_in_fundefs_bound_var_fundefs. now eauto. }
@@ -1480,15 +1568,18 @@ Section Inline_correct.
            rewrite Dom_map_def_funs. eapply Union_Disjoint_r.
            ++ eapply Disjoint_Included_r. eapply name_in_fundefs_bound_var_fundefs. sets.
            ++ sets.
+        -- eapply Disjoint_Included_r. eapply image_apply_r_set_list; eauto. eapply Union_Disjoint_r. now sets.
+           rewrite Dom_map_def_funs. rewrite <- Same_set_all_fun_name. rewrite Setminus_Union_distr.
+           rewrite Setminus_Same_set_Empty_set. repeat normalize_sets. now sets.
         -- eapply fun_map_inv_antimon. rewrite <- Hseq. rewrite <- H12. eapply fun_map_inv_def_funs.
            eapply fun_map_inv_i_mon. eassumption. omega. rewrite H12, Hseq. eapply preord_env_P_inj_antimon.
            eassumption. normalize_occurs_free. now sets. eassumption. normalize_occurs_free. sets.
            repeat normalize_bound_var_in_ctx. now sets. 
            
-           eapply Disjoint_Included; [ | | eapply Hdis3 ]. now sets. admit.
-           eapply Disjoint_Included_l. eapply Included_trans. eapply name_in_fundefs_bound_var_fundefs. eassumption.
-           eapply Disjoint_Included; [| | eapply Hdis2 ]. rewrite image_Union. now sets.
-           intros z Hin. eapply Hf. unfold Ensembles.In, Range in *. zify. omega.
+           eapply Disjoint_Included_l; [ | eapply Hdis' ].
+           eapply Included_trans. rewrite Same_set_all_fun_name, H12, Hseq. eassumption.
+           intros z Hin. eapply Hf. unfold Range, Ensembles.In in Hin. zify. omega. 
+
            normalize_occurs_free. rewrite !Union_assoc. rewrite Union_Setminus_Included. now sets. tci. now sets.
     - (* Eapp *)
       simpl. destruct (update_App St IH (apply_r sig v) t (apply_r_list sig l) st) as [s b] eqn:Hup. 
@@ -1510,7 +1601,7 @@ Section Inline_correct.
           -- destruct (Datatypes.length xs =? Datatypes.length l)%nat eqn:Hbeq.
              { symmetry in Hbeq. eapply beq_nat_eq in Hbeq.      
                edestruct Hfm. eassumption. destructAll. eapply post_weakening; [| eapply IHd ].
-               ++ simpl. intros. destructAll. 
+               ++ simpl. intros. destructAll.  
                   split; [| split; [| split; [| split; [| split ]]]]; try eassumption.
                   ** eapply Included_trans. eassumption. 
                      eapply Included_trans. eapply image_apply_r_set_list.
@@ -1523,16 +1614,24 @@ Section Inline_correct.
                   ** intros. eapply preord_exp_app_l.
                      --- admit. (* post *)
                      --- admit. (* post *) 
-                     --- intros. assert (Hf := H14). assert (Heqf' := Heqf). edestruct H14; eauto. destructAll.
-                         do 2 subst_exp. eapply H11.
-                         +++ edestruct preord_env_P_inj_get_list_l. now eapply H12. normalize_occurs_free. now sets.
+                     --- intros. assert (Hf := H16). assert (Heqf' := Heqf). edestruct H16; eauto. destructAll.
+                         do 2 subst_exp. eapply H12.
+                         +++ edestruct preord_env_P_inj_get_list_l. now eapply H13. normalize_occurs_free. now sets.
                              eassumption. destructAll.                           
                              eapply preord_env_P_inj_set_lists_l'; try eassumption.
                          +++ erewrite Dom_map_set_lists; [| eassumption ]. rewrite Dom_map_def_funs. xsets.
                              eapply Union_Disjoint_r; xsets. eapply Disjoint_Included_r; [| eapply H1 ]. sets.
+                         +++ rewrite Dom_map_set_lists; eauto. eapply Disjoint_Included_r.
+                             eapply image_apply_r_set_list. unfold apply_r_list. rewrite map_length. now eauto.
+                             rewrite Setminus_Union_distr. rewrite Setminus_Same_set_Empty_set. repeat normalize_sets.
+                             eapply Union_Disjoint_r.
+                             *** eapply Disjoint_Included_r; [| eapply Hdis2 ].
+                                 normalize_occurs_free. rewrite image_Union. rewrite FromList_apply_list. sets.
+                             *** eapply Disjoint_Included_r. eapply image_monotonic. eapply Included_Setminus_compat.
+                                 eapply Dom_map_sub_map. eassumption. reflexivity. sets.
                          +++ eapply fun_map_inv_antimon. eapply fun_map_inv_set_lists; [ | | | eassumption ].
-                             *** eapply fun_map_inv_sig_extend_Disjoint. rewrite <- fun_map_inv_eq in *. eapply H25.
-                                 eapply Disjoint_Included_r; [| eapply H3 ]. sets.
+                             *** eapply fun_map_inv_sig_extend_Disjoint. rewrite <- fun_map_inv_eq in *. eassumption.
+                                 rewrite Dom_map_def_funs. sets.
                              *** eassumption.
                              *** rewrite Dom_map_def_funs. eapply Union_Disjoint_r. now sets. 
                                  clear H24. xsets.
@@ -1545,10 +1644,9 @@ Section Inline_correct.
                   unfold apply_r_list. rewrite list_length_map. eassumption.
                   eapply Union_Disjoint_r.
                   eapply Disjoint_Included_r; [| eapply Hdis2 ]. normalize_occurs_free.
-                  rewrite image_Union. rewrite FromList_apply_list. now sets.
-                  rewrite Setminus_Union_distr. now xsets.
+                  rewrite image_Union. rewrite FromList_apply_list. now sets. now sets.
                ++ sets.
-               ++ s
+               ++ sets.
                ++ (* Make lemma if needed about fun_map_vars fm S (set_list (combine xs (apply_r_list sig l)) sig) *)
                   intros ? ? ? ? ?. edestruct Hfm; eauto. destructAll.
                   repeat (split; [ now eauto |]). eapply Union_Disjoint_r. now sets.
@@ -1597,4 +1695,138 @@ Section Inline_correct.
       admit.
     - (* Ehalt *)
       admit.
+    - (* Fcons *)
+      simpl. 
+      eapply bind_triple. eapply pre_transfer_r. now eapply get_names_lst_fresh. intros xs w. simpl.
+      eapply pre_curry_l. intros Hf. eapply pre_curry_l. intros Hnd.  eapply pre_curry_l. intros Hlen.
+      eapply bind_triple. 
+      { do 2 eapply frame_rule. eapply IHe with (S := S \\ FromList xs).
+        - eassumption.
+        - eapply fun_in_fundefs_Disjoint_bound_Var_occurs_free; [| | eassumption ]. now left.
+          constructor; eauto.
+        - eapply Union_Disjoint_r. repeat normalize_bound_var_in_ctx. now xsets.
+          eapply Disjoint_Included_r. eapply image_apply_r_set_list. now eauto.
+          eapply Union_Disjoint_r. now sets.
+          eapply Disjoint_Included; [| | eapply Hdis2 ]; [| now sets ].
+          eapply Included_Union_preserv_r. eapply image_monotonic.
+          eapply Setminus_Included_Included_Union. eapply Included_trans. eapply occurs_free_in_fun.
+          2:{ now sets. } now left.
+        - eapply Disjoint_Included_l; [| eassumption ].
+          normalize_bound_var. simpl. admit. (* same ? *)
+        - repeat normalize_occurs_free_in_ctx. repeat normalize_bound_var_in_ctx. 
+          sets.
+        - repeat normalize_occurs_free_in_ctx. repeat normalize_bound_var_in_ctx.
+          admit. (* fun_map_vars set_list *) }
+      intros e' w'. simpl. eapply pre_curry_l. intros Hxs. eapply pre_curry_l; intros Hleq.     
+      eapply bind_triple.
+
+      { eapply pre_strenghtening.
+        2:{ eapply frame_rule. eapply IHB with (S := S \\ FromList xs (* \\ bound_var e' *)).
+            + eassumption.
+            + repeat normalize_bound_var_in_ctx. repeat normalize_occurs_free_in_ctx.
+              eapply Disjoint_Included_r. eapply Included_Union_Setminus with (s2 := [set v]). now tci.
+              eapply Union_Disjoint_r. eapply Disjoint_Included; [| | eapply Hdis1 ]; now sets.
+              sets.
+            + repeat normalize_bound_var_in_ctx. repeat normalize_occurs_free_in_ctx.
+              eapply Union_Disjoint_r. now xsets.
+              eapply Disjoint_Included; [| | eapply Hdis2 ]. eapply Included_Union_preserv_r.
+              eapply image_monotonic. rewrite <- Union_assoc. rewrite <- Union_Included_Union_Setminus with (s3 := [set v]).
+              sets. tci. sets. sets.
+            + repeat normalize_bound_var_in_ctx. repeat normalize_occurs_free_in_ctx.
+              eapply Disjoint_Included_l; [| eapply Hdis3 ]. simpl. rewrite !Setminus_Union_distr.
+              do 3 eapply Included_Union_preserv_r. rewrite !Setminus_Union.
+              rewrite (Union_commut (funname_in_exp e)). rewrite <- !Union_assoc. rewrite (Union_commut [set v]). 
+              rewrite Union_assoc. rewrite <- Union_assoc. rewrite <- Setminus_Union. rewrite <- Setminus_Union.
+              eapply Included_Setminus; [| now sets ]. eapply Union_Disjoint_r.
+              * eapply Disjoint_Included_r. eapply funname_in_exp_subset. sets.
+              * sets.
+            + sets.
+            + admit. (* fun_map_vars S mon *) }
+        simpl. intros u w1 [Hyp Hyp']. split. eapply Hyp'. eassumption. }
+
+
+      intros B' w''. eapply return_triple. intros. destructAll. split; [| split ; [| split; [| split; [| split; [| split ]]]]].
+      + eapply fresh_monotonic; [|  eassumption ]. sets.
+      + zify; omega.
+      + constructor; eauto.
+        * intros Hc. eapply Hdis2. constructor. 2:{ right. eapply In_image. right. now left. }
+          eapply Hf. eapply H18 in Hc. unfold Ensembles.In, Range in Hc. zify; omega.
+        * intros Hc. eapply Included_Union_Setminus with (s2 := name_in_fundefs B') in Hc; [| tci ].
+          inv Hc. 
+          -- eapply Hdis2. constructor. 2:{ right. eapply In_image. right. now left. }
+             eapply Hf. eapply H13 in H20. unfold Ensembles.In, Range in H20. zify; omega.
+          -- rewrite Same_set_all_fun_name in H20. rewrite H14 in H20. rewrite FromList_apply_list in H20. 
+             admit. (* NODUP *)
+             
+        * eapply Disjoint_Included. eassumption. eassumption. eapply Disjoint_sym. eapply Disjoint_Range. reflexivity.
+        * admit.
+          (* eapply Disjoint_Included. eassumption. eassumption. eapply Disjoint_sym. eapply Disjoint_Range. zify. omega. *)
+        * admit. 
+          (* eapply Disjoint_Included. eassumption. eassumption. eapply Disjoint_Range. reflexivity. *)
+        * intros Hc. eapply Hdis2. constructor. 2:{ right. eapply In_image. right. now left. }
+          eapply Hf. eapply Hxs in Hc. unfold Ensembles.In, Range in Hc. zify; omega.
+      + normalize_occurs_free. eapply Included_trans. eapply Included_Union_compat.
+        * eapply Included_Setminus_compat. eassumption. reflexivity.
+        * eapply Included_Setminus_compat. eassumption. reflexivity.
+        * eapply Union_Included.
+          -- eapply Included_trans. eapply Included_Setminus_compat. eapply image_apply_r_set_list. now eauto. reflexivity.
+             rewrite !Setminus_Union_distr. eapply Union_Included. now sets.
+             rewrite Same_set_all_fun_name. rewrite H14. rewrite FromList_apply_list. rewrite <- Same_set_all_fun_name.
+             rewrite (Union_commut (FromList xs)). rewrite Union_assoc. rewrite <- Setminus_Union.
+             eapply Included_trans. eapply Setminus_Included. eapply Included_trans.
+             rewrite <- image_Singleton, <- image_Union. eapply image_Setminus. now tci.
+             rewrite !Setminus_Union_distr, !Setminus_Union. normalize_occurs_free.
+             rewrite !image_Union. eapply Union_Included; xsets.
+          -- rewrite <- image_Singleton. eapply Included_trans. eapply image_Setminus. now tci.
+             rewrite Setminus_Union_distr. normalize_occurs_free. sets.             
+      + normalize_bound_var. simpl. rewrite Setminus_Union_distr. eapply Union_Included. now sets.
+        rewrite !Setminus_Union_distr. eapply Union_Included; [| eapply Union_Included ].
+        * eapply Included_trans. eapply Setminus_Included.
+          eapply Included_trans. eassumption. eapply Range_Subset; zify; omega.
+        * eapply Included_trans. eapply Setminus_Included.
+          eapply Included_trans. eassumption. eapply Range_Subset; zify; omega.
+        * rewrite Union_commut. rewrite <- Setminus_Union.
+          eapply Included_trans. eapply Setminus_Included.
+          eapply Included_trans. eassumption. eapply Range_Subset; zify; omega.
+      + simpl. rewrite H14. reflexivity.
+      + intros. destruct (cps.M.elt_eq f v); subst.
+        * inv H20. do 2 eexists. split; [| split; [| split; [| split ]]].
+          -- simpl. rewrite peq_true. reflexivity.
+          -- now eauto.
+          -- eassumption.
+          -- intros z HIn. eapply Hf. eapply Hxs in HIn. unfold Ensembles.In, Range in HIn. zify; omega.
+          -- intros. eapply H19.
+             ++ rewrite apply_r_set_list_f_eq.
+                eapply preord_env_P_inj_antimon. eassumption. eapply Included_trans.
+                eapply occurs_free_in_fun with (B := (Fcons v ft xs0 e1 f5)). now left.
+                sets.
+             ++ sets.
+             ++ rewrite apply_r_set_list_f_eq. eassumption.
+             ++ eapply fun_map_inv_antimon. eassumption.
+                eapply Included_trans. eapply occurs_free_in_fun with (B := (Fcons v ft xs0 e1 f5)). now left.
+                sets.
+        * edestruct H15. eassumption. destructAll.
+          do 2 eexists. split; [| split; [| split; [| split ]]].
+          -- simpl. rewrite peq_false. eassumption. admit. (* HUN *)
+          -- now eauto.
+          -- eassumption.
+          -- eapply Included_trans. eassumption. sets.
+          -- intros. eapply H25; eauto.
+             ++ eapply preord_env_P_inj_antimon. eassumption. normalize_occurs_free.
+                rewrite <- !Union_assoc.
+                rewrite <- Union_Included_Union_Setminus with (s1 := occurs_free_fundefs _) (s3 := [set v]).
+                now sets. tci. now sets.
+             ++ sets.
+             ++ eapply fun_map_inv_antimon. eassumption. normalize_occurs_free. 
+                rewrite <- !Union_assoc.
+                rewrite <- Union_Included_Union_Setminus with (s1 := occurs_free_fundefs _) (s3 := [set v]).
+                now sets. tci. now sets.
+    - (* Fnil *)
+      eapply return_triple.
+      intros. split; [| split; [| split; [| split; [| split; [| split ]]]]]; eauto.
+      + reflexivity.
+      + constructor.
+      + intros z Hin; inv Hin.
+      + normalize_bound_var. sets.
+      + intros. inv H0.
   Qed.
